theories/typing/uninit.v
@@ -1,80 +1,58 @@
 Require Import FunctionalExtensionality Equality.
 From iris.proofmode Require Import tactics.
-From lrust.util Require Import types.
+From lrust.util Require Import basic types.
+From lrust.typing Require Import mod_ty array product.
 From lrust.typing Require Export type.
 Set Default Proof Using "Type".
 
 Section uninit.
   Context `{!typeG Σ}.
 
-  Fixpoint uninit_shr n κ l := (match n with 0 => True |
-    S m => (∃v, &frac{κ} (λ q, l ↦{q} v)) ∗ uninit_shr m κ (l +ₗ 1) end)%I.
+  Program Definition uninit1: type unit :=
+    {| pt_size := 1;  pt_own _ _ vl := ⌜∃v, vl = [v]⌝; |}%I.
+  Next Obligation. move=> *. by iDestruct 1 as (?) "->". Qed.
+  Global Instance uninit1_send : Send uninit1. Proof. done. Qed.
 
-  Lemma upd_uninit_shr E vl n κ l : ↑lftN ⊆ E →
-    length vl = n → lft_ctx -∗ &{κ} (l ↦∗ vl) ={E}=∗ uninit_shr n κ l.
+  Definition uninit n : type unit := <{const ()}> (array n uninit1).
+
+  Local Notation tts := (@prepeat id _ ()).
+  Local Lemma pvec_unit_unique n x : x = tts n.
   Proof.
-    move=> ?. move: vl l. elim n; [by iIntros|]=> ? IH [|v?]; [done|]=> > [=?].
-    rewrite heap_mapsto_vec_cons. iIntros "#LFT Bor".
-    iMod (bor_sep with "LFT Bor") as "[Head Tail]"; [done|].
-    iMod (bor_fracture (λ q, _ ↦{q} _)%I with "LFT Head") as "Head"; [done|].
-    iMod (IH with "LFT Tail") as "$"; [done|]. iModIntro. iExists v. iFrame.
+    move: x. elim n=> /=[|? IH] x; [by case x|]. case x=> [[]?]. f_equal. apply IH.
   Qed.
-
-  Program Definition uninit n : type unit := {|
-    ty_size := n;  ty_lfts := [];  ty_E := [];  ty_own _ _ vl := ⌜length vl = n⌝;
-    ty_shr _ κ _ l := uninit_shr n κ l;
-  |}%I.
-  Next Obligation.
-    move=>/= n _ ? _. elim n; [apply _|]=>/= *. apply bi.sep_persistent; apply _.
-  Qed.
-  Next Obligation. by iIntros. Qed. Next Obligation. by iIntros. Qed.
-  Next Obligation. by iIntros. Qed.
-  Next Obligation.
-    move=>/= n ? ? _ _. elim n; [by iIntros|]=> ? IH ?. iIntros "#? [One ?]".
-    iDestruct "One" as (v) "#?". iSplit.
-    { iExists v. by iApply frac_bor_shorten. } by iApply IH.
-  Qed.
-  Next Obligation.
-    move=>/= *. iIntros "#LFT #In Bor Tok".
-    iMod (bor_exists with "LFT Bor") as (vl) "Bor"; [done|].
-    iMod (bor_sep with "LFT Bor") as "[Bor Bor']"; [done|].
-    iMod (bor_persistent with "LFT Bor' Tok") as "[>% ?]"; [done|].
-    iApply step_fupdN_intro; [done|].
-    by iMod (upd_uninit_shr with "LFT Bor") as "$".
-  Qed.
-  Next Obligation.
-    iIntros. iApply step_fupdN_intro; [done|]. iIntros "!>!>!>".
-    iExists [], 1%Qp. iSplit. { iPureIntro. apply proph_dep_unit. }
-    iSplit; [done|]. iIntros "_ !>". by iSplit.
-  Qed.
-  Next Obligation.
-    iIntros. iApply step_fupdN_intro; [done|]. iIntros "!>!>!>!>!>".
-    iExists [], 1%Qp. iSplit. { iPureIntro. apply proph_dep_unit. }
-    iSplit; [done|]. iIntros "_ !>". iFrame.
-  Qed.
-
-  Global Instance uninit_copy n : Copy (uninit n).
+  Local Instance const_tt_tts_iso n : Iso (const ()) (const (tts n)).
   Proof.
-    split; [apply _|]=> ????? l q ? /=. move: l q. elim n=> [|? IH].
-    - move=> *. iIntros "_ _ Na $ !>". iExists 1%Qp, []. rewrite heap_mapsto_vec_nil.
-      iDestruct (na_own_acc with "Na") as "[$ ToNa]"; [solve_ndisj|].
-      do 2 (iSplit; [done|]). iIntros "Na". by iDestruct ("ToNa" with "Na") as "$".
-    - move=> ?? HF.
-      iIntros "#LFT [Bor Shr] Na [Tok Tok']". iDestruct "Bor" as (v) "Bor".
-      iMod (frac_bor_acc with "LFT Bor Tok") as (q) "[>Mt Close]"; [solve_ndisj|].
-      iMod (IH with "LFT Shr Na Tok'") as (q' vl) "[Na[Mt'[>%Eq Close']]]".
-      { move: HF. rewrite -Nat.add_1_l -Nat.add_assoc shr_locsE_shift. set_solver+. }
-      iDestruct (na_own_acc with "Na") as "[$ ToNa]".
-      { rewrite -Nat.add_1_l shr_locsE_shift. set_solver+. }
-      case (Qp_lower_bound q q')=> [q''[?[?[->->]]]]. iModIntro. iExists q'', (v :: vl).
-      rewrite heap_mapsto_vec_cons. iDestruct "Mt" as "[$ Mtr]".
-      iDestruct "Mt'" as "[$ Mtr']". iSplit. { iPureIntro. by rewrite /= Eq. }
-      iIntros "Na [Mt Mt']". iDestruct ("ToNa" with "Na") as "Na".
-      iMod ("Close" with "[$Mt $Mtr]") as "$".
-      by iMod ("Close'" with "Na [$Mt' $Mtr']") as "[$$]".
+    split; extensionality x; [|by case x]=>/=. symmetry. apply pvec_unit_unique.
   Qed.
 
-  Global Instance uninit_send n : Send (uninit n). Proof. done. Qed.
-  Global Instance uninit_sync n : Sync (uninit n). Proof. done. Qed.
+  Lemma uninit_own' n vπd tid vl :
+    (array n uninit1).(ty_own) vπd tid vl ⊣⊢ ⌜length vl = n⌝.
+  Proof. move: vl vπd. elim: n=> /=[|n IH] vl [vπ ?]; iSplit.
+    - by iIntros ([_[_->]]).
+    - rewrite length_zero_iff_nil. iIntros (->). iExists (const ()). iPureIntro.
+      split; [|done]. extensionality π. simpl. by case (vπ π)=> [].
+    - iDestruct 1 as (? _ ??->[_[_[?->]]]) "H /=". rewrite IH. by iDestruct "H" as %->.
+    - case vl=> /=[|v vl']; iIntros (Eq); [done|]. iExists (const ((), tts n)).
+      iSplit. { iPureIntro. extensionality π. simpl. apply (pvec_unit_unique (S n)). }
+      iExists [v], vl'. rewrite IH. iPureIntro. split; [done|].
+      split; [|by move: Eq=> [=]]. exists (). split; by [|exists v].
+  Qed.
+  Lemma uninit_own n vπd tid vl : (uninit n).(ty_own) vπd tid vl ⊣⊢ ⌜length vl = n⌝.
+  Proof.
+    simpl. setoid_rewrite uninit_own'. iPureIntro. split; [by move=> [_[_->]]|]=> ->.
+    exists (const (tts n)). split; [|done]. extensionality π. by case (vπd.1 π).
+  Qed.
+
+  Lemma uninit_plus_prod E L m n :
+    eqtype E L (const ((), ())) (const ()) (uninit (m + n)) (uninit m * uninit n).
+  Proof.
+    have [->->]: @const _ () ((), ()) =
+        prod_map (const ()) (const ()) ∘ pvsep ∘ const (tts (m + n)) ∧
+      @const _ (() * ()) () =
+        const () ∘ (curry pvapp ∘ prod_map (const (tts m)) (const (tts n))).
+    { split; extensionality x; by [case x|case x=>[[][]]]. }
+    eapply eqtype_trans. { apply mod_ty_outin, _. } eapply eqtype_trans.
+    { apply array_plus_prod. } apply prod_eqtype; apply mod_ty_inout, _.
+  Qed.
 
 End uninit.
